src/lib/GPU.HReduceU32Plus.fsti
@@ -1,18 +1,12 @@
 module GPU.HReduceU32Plus
 
-(* This module is specialized to U64 and addition.
-
-The only admits are a boring fact about associativity of add_mod (unsure why
-it's not already trivial in F* ) and lack of overflow of the iteration counter.
-This last thing should fall out from the fact that any the size of an array must
-fit in a sizet, and the log of that size even more so. *)
-
 #lang-pulse
 
 open GPU
 open GPU.Barrier.RPM
 open GPU.Math
 open GPU.Seq.Common
+open GPU.IsReduction
 
 module A = Pulse.Lib.Array
 module SZ = FStar.SizeT
@@ -22,15 +16,9 @@ let size : sz = 1024sz
 
 (* no polymorphism, but at least keep the definitions here *)
 let ety = u32
-inline_for_extraction noextract let op = U32.add_mod
-inline_for_extraction noextract let neu = 0ul
+inline_for_extraction noextract let op  : ety -> ety -> ety = U32.add_mod
+inline_for_extraction noextract let neu : ety = U32.zero
 
-(* using seq_fold_left op neu directly in pulse code blows up
-in many colorful ways. Probably the refinment of op? Anyway, 
-specialize it here. *)
-let sum (s : seq ety) : GTot ety =
-  seq_fold_left op neu s
-  
 (* Ownership of array r between i and j. The first value of that slice
 is the reduction of all the values in the (original) slice v. *)
 let gpu_pts_to_slice_sum_inner
@@ -44,7 +32,7 @@ let gpu_pts_to_slice_sum_inner
   ** pure (i < j /\ j <= sz /\
            Seq.length v = sz /\
            Seq.length s = j - i /\
-           Seq.index s 0 == sum (Seq.slice v i j))
+           squash (is_reduction neu op (Seq.slice v i j) (Seq.index s 0))) // SQUASH VERY IMPORTANT!!
 
 let gpu_pts_to_slice_sum
   (#sz:nat)
